spec: replace abstract operator F with procedure; remove unused lemmas

proof/spec/Hash.ec
@@ -19,6 +19,7 @@ op Hash : W8.t list -> W8.t list.
 
 op prf_padding_val : W64.t.
 op prf_kg_padding_val : W64.t.
+op F_padding_val : W64.t.
 op padding_len : int.
 
 module Hash = {
@@ -49,6 +50,20 @@ module Hash = {
     return r;
 
   }
+
+  (* Here, t is nbytesxor tmp bitmask *)
+  proc _F (key t : nbytes) : nbytes = {
+    var r : nbytes;
+    var buf : W8.t list;
+    var padding : W8.t list;
+
+    padding <@ Util.w64_to_bytes (F_padding_val, padding_len);
+    buf <- padding ++ key ++ t;
+
+    r <- Hash buf;
+
+    return r;
+  }
 }.
 
 
@@ -58,4 +73,7 @@ lemma prf_ll : islossless Hash.prf
     by proc; wp; call w64_to_bytes_ll.
 
 lemma prf_kg_ll : islossless Hash.prf_keygen
+    by proc; wp ; call w64_to_bytes_ll.
+
+lemma f_ll : islossless Hash._F 
     by proc; wp ; call w64_to_bytes_ll.
